Fixed issue in the definition of the event that a particular state takes a particular value, which would previously instead give us the event that the final state had that value. Completed theorem which simplifies this event in the special case where we referring to the initial state. Completed theorem which allows us to simplify out intersections with the universal event.

ConvolutionalCodes/map_decoder_convolutional_codeScript.sml
@@ -53,7 +53,7 @@ Definition event_state_takes_value_def:
   {(bs : bool list, ns : bool list) | LENGTH bs = n ∧
                                       LENGTH ns = m ∧
                                       encode_recursive_parity_equation_state
-                                      (ps,qs) ts bs = σ
+                                      (ps,qs) ts (TAKE i bs) = σ
   }
 End
 
@@ -1340,7 +1340,7 @@ Proof
   >> gvs[]
   >> Cases_on ‘bs’ >> gvs[encode_recursive_parity_equation_state_sequence_def]
 QED
-        
+
 Theorem event_state_takes_value_zero:
   ∀n m ps qs ts σ.
     event_state_takes_value n m (ps,qs) ts 0 σ =
@@ -1349,12 +1349,22 @@ Theorem event_state_takes_value_zero:
     else
       ∅
 Proof
-  rw[]
-  >> gvs[event_state_takes_value_def]
-  >> rw[EXTENSION] >> EQ_TAC >> rw[]
-  >> 
+  rw[event_state_takes_value_def]
 QED
 
+Theorem event_input_string_starts_with_event_universal[simp]:
+  ∀n m p E.
+    E ∈ events (ecc_bsc_prob_space n m p)
+    ⇒ E ∩ event_universal n m = E ∧ event_universal n m ∩ E = E
+Proof
+  rw[]
+  >> gvs[events_ecc_bsc_prob_space, POW_DEF, SUBSET_DEF]
+  >> rw[EXTENSION] >> EQ_TAC >> rw[]
+  >> (Cases_on ‘x’ >> gvs[]
+      >> last_x_assum drule
+      >> rw[])
+QED
+                               
 (* -------------------------------------------------------------------------- *)
 (* We want to prove:                                                          *)
 (* P(bs,σs,cs) = P(σ_0)P(b_0)P(σ_1c_0|σ_0b_0)P(b_1)P(σ_2c_1|σ_1b_1)...        *)
@@ -1432,7 +1442,7 @@ Proof
       >- (gvs[]
           >> gvs[event_state_sequence_starts_with_sing]
           >> rw[]
-      )
+         )
       >> gvs[event_state_sequence_starts_with_def]
       >> rw[]
      )
